tests/lean/quote_error_pos.lean
@@ -1,0 +1,22 @@
+open tactic
+
+meta def apply_zero_add (a : pexpr) : tactic unit :=
+to_expr `(zero_add %%a) >>= exact
+
+example (a : nat) : 0 + a = a :=
+begin
+  apply_zero_add `(tt), -- Error should be here
+end
+
+/-
+-- This test is stil failing, Lean is reporting an error inside of `[apply ...]
+-- Possible solution: erase position information from quoted terms inside of `[...]
+meta def apply_zero_add2 (a : pexpr) : tactic unit :=
+`[apply zero_add %%a]
+
+example (a : nat) : 0 + a = a :=
+begin
+  apply_zero_add2 `(tt), -- Error should be here
+end
+
+-/
